Iris/Iris/ProofMode/Instances.lean
@@ -925,7 +925,7 @@ instance elimInv_acc_without_close [BI PROP] {X : Type}
     ϕ1 ϕ2 Pinv Pin (M1 M2 : PROP → PROP) α β mγ Q (Q' : X → PROP)
     [h1 : IntoAcc Pinv ϕ1 Pin M1 M2 α β mγ]
     [h2 : ElimAcc ϕ2 M1 M2 α β mγ Q Q'] :
-    ElimInv (ϕ1 ∧ ϕ2) X Pinv Pin α none Q Q' where
+    ElimInv (ϕ1 ∧ ϕ2) X Pinv Pin α false none Q Q' where
   elim_inv := sorry
 
 set_option synthInstance.checkSynthOrder false in
@@ -936,6 +936,6 @@ instance elimInv_acc_with_close [BI PROP] {X : Type}
     [h2 : ∀ R, ElimModal ϕ2 false false (M1 R) R Q Q'] :
     ElimInv (ϕ1 ∧ ϕ2) X Pinv Pin
             α
-            (some (fun x => iprop(β x -∗ M2 ((mγ x).getD emp))))
+            true (some (fun x => iprop(β x -∗ M2 ((mγ x).getD emp))))
             Q (fun _ => Q') where
   elim_inv := sorry
